DynamoDbEncryption/dafny/DynamoDbEncryptionTransforms/src/DynamoDbMiddlewareSupport.dfy
@@ -49,7 +49,8 @@ module DynamoDbMiddlewareSupport {
     attr : string
   )
   {
-    BS.IsSigned(config.itemEncryptor.config.attributeActionsOnEncrypt, attr)
+    var itemEncryptorClient := config.itemEncryptor as DynamoDbItemEncryptor.DynamoDbItemEncryptorClient;
+    BS.IsSigned(itemEncryptorClient.config.attributeActionsOnEncrypt, attr)
   }
 
   // TestConditionExpression fails if a condition expression is not suitable for the
@@ -63,7 +64,7 @@ module DynamoDbMiddlewareSupport {
   )
     : Result<bool, Error>
   {
-    BS.TestConditionExpression(config.itemEncryptor.config.attributeActionsOnEncrypt, expr, attrNames, attrValues)
+    BS.TestConditionExpression(ItemEncryptorClientConfig(config).attributeActionsOnEncrypt, expr, attrNames, attrValues)
     .MapFailure(e => E(e))
   }
 
@@ -78,7 +79,7 @@ module DynamoDbMiddlewareSupport {
   )
     : Result<bool, Error>
   {
-    BS.TestUpdateExpression(config.itemEncryptor.config.attributeActionsOnEncrypt, expr, attrNames, attrValues)
+    BS.TestUpdateExpression(ItemEncryptorClientConfig(config).attributeActionsOnEncrypt, expr, attrNames, attrValues)
     .MapFailure(e => E(e))
   }
 
@@ -86,7 +87,7 @@ module DynamoDbMiddlewareSupport {
   // returning a replacement AttributeMap.
   method AddSignedBeacons(config : ValidTableConfig, item : DDB.AttributeMap)
     returns (output : Result<DDB.AttributeMap, Error>)
-    requires AwsCryptographyDbEncryptionSdkDynamoDbItemEncryptorOperations.ValidInternalConfig?(config.itemEncryptor.config)
+    requires AwsCryptographyDbEncryptionSdkDynamoDbItemEncryptorOperations.ValidInternalConfig?(ItemEncryptorClientConfig(config))
     requires OneSearchValidState(config)
     ensures OneSearchValidState(config)
     modifies OneSearchModifies(config)
@@ -99,7 +100,7 @@ module DynamoDbMiddlewareSupport {
   // returning just the new items.
   method GetEncryptedBeacons(config : ValidTableConfig, item : DDB.AttributeMap, keyId : Util.MaybeKeyId)
     returns (output : Result<DDB.AttributeMap, Error>)
-    requires AwsCryptographyDbEncryptionSdkDynamoDbItemEncryptorOperations.ValidInternalConfig?(config.itemEncryptor.config)
+    requires AwsCryptographyDbEncryptionSdkDynamoDbItemEncryptorOperations.ValidInternalConfig?(ItemEncryptorClientConfig(config))
     requires OneSearchValidState(config)
     ensures OneSearchValidState(config)
     modifies OneSearchModifies(config)
@@ -184,7 +185,7 @@ module DynamoDbMiddlewareSupport {
     ensures OneSearchValidState(config)
     modifies OneSearchModifies(config)
   {
-    var ret := BS.QueryInputForBeacons(config.search, config.itemEncryptor.config.attributeActionsOnEncrypt, req);
+    var ret := BS.QueryInputForBeacons(config.search, ItemEncryptorClientConfig(config).attributeActionsOnEncrypt, req);
     return ret.MapFailure(e => AwsCryptographyDbEncryptionSdkDynamoDb(e));
   }
 
@@ -208,7 +209,7 @@ module DynamoDbMiddlewareSupport {
     ensures OneSearchValidState(config)
     modifies OneSearchModifies(config)
   {
-    var ret := BS.ScanInputForBeacons(config.search, config.itemEncryptor.config.attributeActionsOnEncrypt, req);
+    var ret := BS.ScanInputForBeacons(config.search, ItemEncryptorClientConfig(config).attributeActionsOnEncrypt, req);
     return ret.MapFailure(e => AwsCryptographyDbEncryptionSdkDynamoDb(e));
   }
 
